editted proof of noninterference preservation for progress sensitive case and added progress insensitive case

theories/Secure/SecurityImpExc/SecurityImp2AsmSecurityPres.v
@@ -25,6 +25,10 @@ From ITree Require Import
      Secure.SecurityImp.KTreeFin
      Secure.SecurityImpExc.SecurityImp2AsmCorrectness
      Secure.SecureEqEuttTrans
+     Secure.SecurityImpExc.SecurityImpTypes
+     Secure.SecureEqProgInsens
+     Secure.SecureEqProgInsensFacts
+     Secure.SecurityImpExc.SecurityImpTypesProgInsens
 .
 
 Import ITreeNotations.
@@ -35,45 +39,80 @@ Open Scope monad_scope.
 
 Section SecurityPreservation.
 
-Context (priv : var -> sensitivity).
+Context (Γ : var -> sensitivity).
+Context (l : label).
 
-Definition low_state_equiv : map -> (registers * memory) -> Prop :=
-  fun s '(r, m) => low_map_equiv priv s m.
+Definition labelled_sim : map -> (registers * memory) -> Prop :=
+  fun g_imp g_asm => labelled_equiv Γ l g_imp (snd g_asm).
 
-Definition low_bisimilar {A B : Type} (RAB : A -> B -> Prop) 
+Lemma state_rel_aux:
+  forall (p1 : map * unit) (p2 : registers * memory * fin 1),
+    rcompose (product_rel (labelled_equiv Γ l) eq) (state_invariant TT) p1 p2 ->
+    product_rel labelled_sim TT p1 p2.
+Proof.
+  intros [σ [] ] [ [regs mem] ?] Hcomp. inv Hcomp.
+  destruct r2 as [σ' [] ]. destruct REL1. split; red; auto.
+  cbn. red in REL2. destruct REL2 as [Hst _ ]. cbn in *.
+  assert (labelled_equiv Γ l σ' mem).
+  { red in Hst. do 2 red. intros. auto. }
+  etransitivity; eauto.
+Qed.
+
+Section ProgressSensitive.
+
+Definition labelled_bisimilar {A B : Type} (RAB : A -> B -> Prop) 
            (t1 : itree (impExcE +' stateE +' IOE) A ) (t2 : itree (impExcE +'
  Reg +' Memory +' IOE) B) :=
-  forall (g_imp : map) (g_asm : memory) (l : registers),
-    low_map_equiv priv g_imp g_asm ->
-    eqit_secure sense_preorder priv_exc_io (product_rel low_state_equiv RAB) true true Public (interp_imp t1 g_imp ) (interp_asm t2 (l, g_asm)).
+  forall (g_imp : map) (g_asm : memory) (regs : registers),
+    labelled_equiv Γ l g_imp g_asm ->
+    eqit_secure sense_preorder priv_exc_io (product_rel labelled_sim RAB) true true l (interp_imp t1 g_imp ) (interp_asm t2 (regs, g_asm)).
 
-Lemma compile_preserves_security : forall (p : stmt),
-    low_eqit_secure_impstate true true priv eq (interp_imp (denote_stmt p)) (interp_imp (denote_stmt p)) ->
-    low_bisimilar TT (denote_stmt p) (denote_asm (compile p) f0 ) .
+Lemma compile_preserves_ps_security : forall (c : stmt),
+    label_state_sec_eutt Γ l eq  (interp_imp (denote_stmt c)) (interp_imp (denote_stmt c)) ->
+    labelled_bisimilar TT (denote_stmt c) (denote_asm (compile c) f0 ) .
 Proof.
-  intros p Hsecp. red in Hsecp. red. intros g_imp g_asm l Hs.
-  assert (low_map_equiv priv g_imp g_imp).
-  { red. intros; auto. }
-  (* there exists some g_imp' *)
-  specialize (compile_correct p) as Heutt. do 2 red in Heutt.
-
+  intros s Hsecs. red in Hsecs. red. intros g_imp g_asm regs Hs.
+  assert (labelled_equiv Γ l g_imp g_imp). reflexivity.
+  specialize (compile_correct s) as Heutt. do 2 red in Heutt.
   assert (Renv g_asm g_asm). reflexivity.
-  specialize (Hsecp g_imp g_asm Hs).
-  specialize (Heutt g_asm g_asm l H0) .
+  specialize (Hsecs g_imp g_asm Hs).
+  specialize (Heutt g_asm g_asm regs H0) .
   specialize (eutt_secure_eqit_secure) as Htrans.
   eapply Htrans in Heutt; eauto.
   eapply SecureEqEuttHalt.eqit_secure_RR_imp; try apply Heutt.
-  (* show that low_map_equiv ∘ Renv <= low_map_equiv *)
-  clear -priv.
-  intros [g_imp ?] [ [l g_asm] ?] Hcomp.
-  split.
-  2 : { red. auto. }
-  cbn. inv Hcomp. red in REL1. cbn in *.
-  destruct r2 as [g_imp' ? ]. destruct REL1 as [REL1 _ ].
-  cbn in *. red in REL2. cbn in *. destruct REL2 as [REL2 _ ].
-  red. intros. red in REL1. red in REL2. rewrite <- REL2.
-  apply REL1; auto.
+  apply state_rel_aux; auto.
 Qed.
+End ProgressSensitive.
+
+Section ProgressInsensitive.
+
+Definition labelled_pi_bisimilar {A B : Type} (RAB : A -> B -> Prop) 
+           (t1 : itree (impExcE +' stateE +' IOE) A ) (t2 : itree (impExcE +'
+ Reg +' Memory +' IOE) B) :=
+  forall (g_imp : map) (g_asm : memory) (regs : registers),
+    labelled_equiv Γ l g_imp g_asm ->
+    pi_eqit_secure sense_preorder priv_exc_io (product_rel labelled_sim RAB) true true l (interp_imp t1 g_imp ) (interp_asm t2 (regs, g_asm)).
+
+Lemma compile_preserves_pi_security : forall (c : stmt),
+    label_state_pi_sec_eutt Γ l eq  (interp_imp (denote_stmt c)) (interp_imp (denote_stmt c)) ->
+    labelled_pi_bisimilar TT (denote_stmt c) (denote_asm (compile c) f0 ) .
+Proof.
+  intros s Hsecs. red in Hsecs. red. intros g_imp g_asm regs Hs.
+  assert (labelled_equiv Γ l g_imp g_imp). reflexivity.
+  specialize (compile_correct s) as Heutt. do 2 red in Heutt.
+  assert (Renv g_asm g_asm). reflexivity.
+  specialize (Hsecs g_imp g_asm Hs).
+  specialize (Heutt g_asm g_asm regs H0) .
+  Locate proper_eutt_pi_secure_eutt.
+  specialize (pi_eqit_secure_mixed_trans) as Htrans.
+  eapply Htrans in Heutt; eauto.
+  eapply pi_eqit_secure_RR_imp; try apply Heutt.
+  apply state_rel_aux; auto.
+Qed.
+
+
+End ProgressInsensitive.
+
   
 End SecurityPreservation.
 (*
